## 5.3 The Convex Conjugate

^0a5cd2

> **Definition 16.1** (*Convex conjugate*).
> Let $F$ be an extended-valued function. Then its *convex conjugate* or *Fenchel dual* $F^\ast: \mathbb R^N \to (-\infty, \infty]$ is defined by
> $$F^\ast(y) = \sup_{x \in \mathbb R^N} \left(\langle x, y\rangle - F(x)\right)$$

- $F^\ast$ is always a convex function, regardless of $F$ being convex
- We directly get the *Fenchel-Young inequality* $$\langle x, y \rangle \leq F(x) + F^\ast(y)$$ ^d415ba

> **Proposition 16.2** (*Properties of the convex conjugate*)
> Let $F: \mathbb R^N \to (-\infty, \infty]$
> 1. $F^\ast$ is lower semicontinuous.
> 2. The *biconjugate* $F^{\ast\ast}$ is the *largest* *lower semicontinuous function* satisfying $F^{\ast\ast}(x) \leq F(x)$ for all $x$. **In particular, if $F$ is convex and lower semicontinuous, $F^{\ast\ast} = F$**. ^e536c6
> 3. For $\tau \neq 0$ define $F_\tau(x) := F(\tau x)$. Then $(F_\tau)^\ast(y) = F^\ast(\tfrac{y}{\tau})$.
> 4. If $\tau > 0$, $(\tau F)^\ast(y) = \tau F^\ast(\tfrac{y}{\tau})$.
> 5. For $z \in \mathbb R^N$ let $F^{(z)} := F(x-z)$. Then $(F^{(z)})^\ast(y) = \langle z, y \rangle + F^\ast(y)$.
^ec92f9


Because of property [[#^e536c6|2.]], the biconjugate $F^{\ast\ast}$ is sometimes called the *convex relaxation* of $F$.

##### Example: computing the convex conjugate
Consider $F(x) = ||x||_2^2/2$. Then $F^\ast(y) = F(y)$ #TODO calculate this!
$$F^\ast(y) = \sup_x (\langle x, y \rangle - ||x||_2^2/2) = \sup_x \langle x, y-x/2\rangle ) = \dots$$

##### Example: conjugate of $\exp$
Let $F(x) = \exp(x)$. The map $x \mapsto xy - \exp(x)$ has a maximum at $x = \ln(y)$ if $y > 0$, so
$$F^\ast(y) = \begin{cases} y \ln y - y, & y > 0 \\ 0, & y = 0 \\ \infty & y < 0\end{cases}$$
This gives rise to *Young's inequality*: $$xy \leq e^x + y \ln(y) - y ~\qquad \forall y>0, x$$